Examples/PaxosFOL.lean
@@ -1,0 +1,176 @@
+import LeanSts.State
+import LeanSts.TransitionSystem
+import LeanSts.Auto
+import Mathlib.Tactic
+
+-- Based on: https://github.com/aman-goel/ivybench/blob/master/paxos/ivy/oopsla17_paxos.ivy
+-- See also: https://github.com/aman-goel/ivybench/blob/master/paxos/ivy/Paxos.ivy
+-- See also: https://github.com/nano-o/ivy-proofs/blob/master/paxos/paxos.ivy
+
+section Paxos
+class BoundedTotalOrder (t : Type) :=
+  -- relation: total order
+  le (x y : t) : Bool
+  negative_one : t
+  maximum : t
+  -- axioms
+  le_refl       (x : t) : le x x
+  le_trans  (x y z : t) : le x y → le y z → le x z
+  le_antisymm (x y : t) : le x y → le y x → x = y
+  le_total    (x y : t) : le x y ∨ le y x
+  le_neg_one  (x : t)   : le negative_one x
+  le_max      (x : t)   : le x maximum
+
+class Quorum (node : Type) (quorum : outParam Type):=
+  -- relation
+  member (a : node) (q : quorum) : Bool
+  -- axioms
+  quorum_intersection :
+    ∀ (q1 q2 : quorum), ∃ (a : node), member a q1 ∧ member a q2
+
+variable {value : Type} [DecidableEq value]
+variable {node : Type} [DecidableEq node]
+variable {round : Type} [DecidableEq round] [BoundedTotalOrder round]
+variable {quorum : Type} [DecidableEq quorum] [Quorum node quorum]
+
+structure Structure :=
+  -- Phase 1(a): a proposer selects a proposal number (ballot) `r` and sends a
+  -- _prepare_ request (`msg_1a`) with number `r` to a majority of acceptors
+  msg_1a (r : round) : Bool
+
+  -- Phase 1(b) : if an acceptor `a` receives a _prepare_ request with number `r`
+  -- greater than that of ANY _prepare_ request to which it has already responded
+  -- then it responds to the request with a promise not to accept any more
+  -- proposals numbered less than `r` AND with the highest-numbered proposal (if
+  -- any) that it has accepted (`max_round` and `max_val`) i.e. `msg_1b`
+  -- equivalent to `one_b_max_vote` in the original Ivy spec
+  msg_1b (a : node) (r : round) (max_round : round) (max_val : value) : Bool
+
+  -- Phase 2(a): if the proposer receives a response to its _prepare_ requests
+  -- (numbered `r`) from a majority/quorum of acceptors, then it sends an _accept_
+  -- request to each of those acceptorsfor a proposal numbered `r` with a
+  -- value `v`, where `v` is the value of the highest-numbered proposal among
+  -- the responses, or is any value if trhe responses reported no proposals
+  msg_2a (r : round) (v : value) : Bool -- also called "proposal"
+
+  -- Phase 2(b): if an acceptor `a` receives an _accept_ request for a proposal
+  -- numbered `r`, it accepts the proposal UNLESS it has already responded
+  -- to a _prepare_ request having a number greater than `r`
+  msg_2b (a : node) (r : round) (v : value) : Bool -- also called "vote"
+
+  -- Got 2(b) from a quorum
+  decision (a : node) (r : round) (v : value) : Bool
+
+
+-- equivalent to `one_b` in the original Ivy spec
+def exists1B (st : @Structure value node round) (n : node) (r : round) : Prop :=
+  ∃ (rmax : round) (v : value), st.msg_1b n r rmax v
+
+-- (ghost) relation left_rnd(N:node, R:round) # := exists R2, RMAX, V. ~le(R2,R) & one_b_max_vote(N,R,RMAX,V)
+def leftRound (st : @Structure value node round) (n : node) (r : round) : Prop :=
+  ∃ (r2 : round) (rmax : round) (v : value),
+    ¬ BoundedTotalOrder.le r2 r ∧
+    st.msg_1b n r rmax v
+
+-- find the maximal vote in a round less than r
+-- assume ((maxr = negone & forall MAXR:round,V:value. ~(~le(r,MAXR) & vote(n,MAXR,V))) |
+--         (maxr ~= negone & ~le(r,maxr) & vote(n,maxr,v) &
+--         (forall MAXR:round,V:value. (~le(r,MAXR) & vote(n,MAXR,V)) -> le(MAXR,maxr))
+--         ));
+def maximalVote (st : @Structure value node round) (n : node) (r : round) (maxr : round) (maxv : value) : Prop :=
+  -- uninitialised, i.e. there are no votes at valid round numbers
+  (maxr = BoundedTotalOrder.negative_one ∧
+    (∀ (MAXR : round) (V : value), ¬ (¬ BoundedTotalOrder.le r MAXR ∧ st.msg_2b n MAXR V))) ∨
+  -- (current) r > maxr AND there is a vote for (maxr, maxv) AND
+  -- every other vote is at a lower round number than `maxr`
+  (maxr ≠ BoundedTotalOrder.negative_one ∧
+    ¬ BoundedTotalOrder.le r maxr ∧
+    st.msg_2b n maxr maxv ∧
+    (∀ (MAXR : round) (V : value), (¬ BoundedTotalOrder.le r MAXR ∧ st.msg_2b n MAXR V) → BoundedTotalOrder.le MAXR maxr)
+  )
+
+def chosenAt (st : @Structure value node round) (r : round) (v : value) : Prop :=
+  ∃ (q : quorum), ∀ (n : node), Quorum.member n q → st.decision n r v
+
+-- quorum that shows (rin, vin) is safe
+def showsSafeAt (st : @Structure value node round) (qin : quorum) (rin : round) (vin : value): Prop :=
+  -- a majority of acceptors have joined round `rin`
+  (∀ (N : node), Quorum.member N qin → exists1B st N rin) ∧
+  -- and either
+  (∃ (MAXRIn : round),
+    -- nothing has happened; FIXME: why does this exist?
+    (MAXRIn = BoundedTotalOrder.negative_one ∧
+      (∀ (N : node) (MAXR : round) (V : value),
+        ¬ (Quorum.member N qin ∧ ¬ BoundedTotalOrder.le rin MAXR ∧ st.msg_2b N MAXR V))) ∨
+    -- OR ∃ node in the quorum that voted for the value at some previous round MAXRIn, AND
+    -- MAXRIn is the largest round number in the quorum that voted for the value
+    (MAXRIn ≠ BoundedTotalOrder.negative_one ∧
+      (∃ (N : node), Quorum.member N qin ∧ ¬ BoundedTotalOrder.le rin MAXRIn ∧ st.msg_2b N MAXRIn vin) ∧
+      (∀ (N : node) (MAXR : round) (V : value),
+        (Quorum.member N qin ∧ ¬ BoundedTotalOrder.le rin MAXR ∧ st.msg_2b N MAXR V) → BoundedTotalOrder.le MAXR MAXRIn)
+    )
+  )
+
+def isSafeAt (st : @Structure value node round) (r : round) (v : value) : Prop :=
+  ∃ (q : quorum), showsSafeAt st q r v
+
+def initialState? (st : @Structure value node round) : Prop :=
+  (∀ (r : round), ¬ st.msg_1a r) ∧
+  (∀ (n : node) (r1 r2 : round) (v : value), ¬ st.msg_1b n r1 r2 v) ∧
+  (∀ (r : round) (v : value), ¬ st.msg_2a r v) ∧
+  (∀ (n : node) (r : round) (v : value), ¬ st.msg_2b n r v) ∧
+  (∀ (n : node) (r : round) (v : value), ¬ st.decision n r v)
+
+-- a proposer selects a round and sends a message asking nodes to join the round
+@[simp] def phase_1a : RelationalTransitionSystem.action (@Structure value node round) :=
+  λ (st st' : @Structure value node round) =>
+    ∃ (r : round),
+      -- preconditions
+      r ≠ BoundedTotalOrder.negative_one ∧
+      -- update
+      st' = { st with msg_1a := st.msg_1a[r ↦ true] }
+
+-- "join round" = receive 1a and answer with 1b
+@[simp] def phase_1b : RelationalTransitionSystem.action (@Structure value node round) :=
+  λ (st st' : @Structure value node round) =>
+    ∃ (n : node) (r : round) (max_round : round) (max_val : value),
+      -- preconditions
+      r ≠ BoundedTotalOrder.negative_one ∧
+      st.msg_1a r ∧
+      ¬ leftRound st n r ∧
+      maximalVote st n r max_round max_val ∧ -- find the maximal vote in a round less than `r`
+      -- update
+      st' = { st with msg_1b := st.msg_1b[n, r, max_round, max_val ↦ true] }
+      -- NOTE: one_b and left_rnd are ghost relations which we don't update
+
+-- "propose" = receive a quorum of 1b's and send a 2a (proposal)
+@[simp] def phase_2a : RelationalTransitionSystem.action (@Structure value node round) :=
+  λ (st st' : @Structure value node round) =>
+    ∃ (r : round) (v : value),
+      -- preconditions
+      r ≠ BoundedTotalOrder.negative_one ∧
+      (forall (V : value), ¬ st.msg_2a r V) ∧
+      isSafeAt st r v ∧
+      -- update
+      st' = { st with msg_2a := st.msg_2a[r, v ↦ true] }
+
+-- "cast vote" = receive a 2a and send 2b
+@[simp] def phase_2b : RelationalTransitionSystem.action (@Structure value node round) :=
+  λ (st st' : @Structure value node round) =>
+    ∃ (n : node) (r : round) (v : value),
+      -- preconditions
+      r ≠ BoundedTotalOrder.negative_one ∧
+      ¬ leftRound st n r ∧
+      st.msg_2a r v ∧
+      -- update
+      st' = { st with msg_2b := st.msg_2b[n, r, v ↦ true] }
+
+-- "decide" = receive a quorum of 2b's
+@[simp] def decision : RelationalTransitionSystem.action (@Structure value node round) :=
+  λ (st st' : @Structure value node round) =>
+    ∃ (n : node) (r : round) (v : value),
+      -- preconditions
+      r ≠ BoundedTotalOrder.negative_one ∧
+      chosenAt st r v ∧
+      -- update
+      st' = { st with decision := st.decision[n, r, v ↦ true] }
